coq: ZF: refactor

coq/ZF/Class/Isom.v
@@ -7,17 +7,18 @@ Require Import ZF.Set.Eval.
 Require Import ZF.Set.OrdPair.
 
 (* H is an isomorphism from A to B w.r. to R and S.                             *)
-Definition Isom (H R S A B:Class) : Prop := Bij H A B /\ forall x y, A x -> A y ->
-  R :(x,y): <-> S :(H!x,H!y):.
+Definition Isom (F R S A B:Class) : Prop := Bij F A B /\ forall x y, A x -> A y ->
+  R :(x,y): <-> S :(F!x,F!y):.
 
-Proposition ConverseIsIsom : forall (H R S A B:Class),
-  Isom H R S A B -> Isom H^:-1: S R B A.
+Proposition ConverseIsIsom : forall (F R S A B:Class),
+  Isom F R S A B -> Isom F^:-1: S R B A.
 Proof.
-  intros H R S A B [H1 H2]. split.
+  intros F R S A B [H1 H2]. split.
   - apply ConverseIsBij. assumption.
   - intros x y H3 H4. split; intros H5.
     + apply H2.
-      * apply BijConverseEvalIsInDomain with B; assumption.
-      * apply BijConverseEvalIsInDomain with B; assumption.
+      * apply BijF_EvalIsInDomain with B; assumption.
+      * apply BijF_EvalIsInDomain with B; assumption.
       *
+
 Admitted.
